case-studies/revolvingDoor/Extra2.thy
@@ -1,0 +1,101 @@
+theory Extra2
+  imports ExtraInv VCTheoryLemmas
+begin
+ 
+theorem "VC2 extraInv env s0 user_value pressure_value"
+  apply(simp only: VC2_def extraInv_def)
+  apply(rule impI)
+  apply(rule conjI)
+   apply simp
+  apply((drule conjE)+)
+                   prefer 18
+                   apply assumption
+                  prefer 17
+                  apply assumption
+                 prefer 16
+                 apply assumption
+                prefer 15
+                apply assumption
+               prefer 14
+               apply assumption
+              prefer 13
+              apply assumption
+             prefer 12
+             apply assumption
+            prefer 11
+            apply assumption
+           prefer 10
+           apply assumption
+          prefer 9
+          apply assumption
+         prefer 8
+         apply assumption
+        prefer 7
+        apply assumption
+       prefer 6
+       apply assumption
+      prefer 5
+      apply assumption
+     prefer 4
+     apply assumption
+  prefer 3
+    apply assumption
+   prefer 2
+   apply assumption
+  subgoal premises prems
+    apply(rule conjI)
+    using prems(1-5) prems(6) apply simp
+    apply(rule conjI)
+    using prems(1-5) prems(7) apply simp
+    apply(rule conjI)
+    using prems(1-5) prems(8) apply simp
+     apply(rule conjI)
+    using prems(1-5) prems(9) apply simp
+     apply blast
+    apply(rule conjI)
+    using prems(1-5) prems(10) apply simp
+    apply(rule conjI)
+    using prems(1-5) prems(11) apply simp
+    apply(rule conjI)
+using prems(1-5)  prems(12) apply simp
+     apply(rule exI[of _ s0])
+     apply simp
+     apply(rule exI[of _ "toEnv (setPstate (setVarBool (setVarAny s0 True True) brake True) user Controller'suspended)"])
+  using substate_refl toEnvNum_id apply simp
+  apply(rule conjI)
+   apply((rule allI)+)
+   apply(rule impI)
+  using prems(1-5) apply(simp split: if_splits)
+    apply(rule cut_rl[of "(toEnv (setPstate (setVarBool (setVarAny s0 True True) brake True) user Controller'suspended))  = s0"])
+     apply simp
+    apply(rule cut_rl[of "substate s0 (toEnv (setPstate (setVarBool (setVarAny s0 True True) brake True) user Controller'suspended)) "])
+  using substate_trans substate_asym apply blast
+  using substate_refl apply simp
+   apply(simp only: One_nat_def[symmetric])
+  using prems(13) apply simp
+   apply blast
+  apply(rule conjI)
+   apply(rule allI)
+  apply(rule impI)
+  using prems(1-5) apply (simp split: if_splits)
+ apply(rule exI[of _ s0])
+    apply simp
+ apply(rule exI[of _ "(toEnv (setPstate (setVarBool (setVarAny s0 user_value pressure_value) brake True) ERROR Controller'suspended)) "])
+  apply simp
+    apply (metis substate.simps(10) substate.simps(2) substate.simps(3) substate.simps(9) substate_asym substate_refl toEnvNum_id)
+  using prems(14) apply auto[1]
+  apply(rule conjI)
+  using prems(1-5) prems(15) apply simp
+  apply(rule conjI)
+  using prems(1-5) prems(16) apply simp
+  apply(rule conjI)
+   apply(rule allI)
+   apply(rule impI)
+  using prems(1-5) apply (simp split: if_splits)
+  using substate_refl prems(15) apply auto[1]
+  using prems(17) apply auto[1]
+  using prems(1-5) prems(18) by simp
+  done
+
+end
+   
