case-studies/revolvingDoor/Extra4.thy
@@ -1,0 +1,119 @@
+theory Extra4
+  imports ExtraInv VCTheoryLemmas
+begin
+
+theorem extra4: "VC4 extraInv env s0 user_value pressure_value"
+  apply(simp only: VC4_def extraInv_def)
+  apply(rule impI)
+  apply(rule conjI)
+   apply simp
+  apply((drule conjE)+)
+                  prefer 17
+                  apply assumption
+                 prefer 16
+                 apply assumption
+                prefer 15
+                apply assumption
+               prefer 14
+               apply assumption
+              prefer 13
+              apply assumption
+             prefer 12
+             apply assumption
+            prefer 11
+            apply assumption
+           prefer 10
+           apply assumption
+          prefer 9
+          apply assumption
+         prefer 8
+         apply assumption
+        prefer 7
+        apply assumption
+       prefer 6
+       apply assumption
+      prefer 5
+      apply assumption
+     prefer 4
+     apply assumption
+    prefer 3
+    apply assumption
+   prefer 2
+   apply assumption
+  subgoal premises prems
+    apply(rule conjI)
+     apply(rule allI)
+     apply(rule impI)
+    subgoal for s1
+      apply(cases "s1=(toEnv (setVarAny s0 user_value pressure_value))")
+    using prems(1-4) prems(5) apply -
+      apply(drule allE[of _ s0])
+       prefer 2
+       apply assumption
+      apply(drule impE)
+    using  substate_refl apply simp
+       prefer 2
+       apply assumption
+      apply(drule disjE)
+        prefer 3
+        apply assumption
+       apply(rule disjI1)
+      apply simp
+      apply(rule disjI2)
+      apply(drule exE)
+       prefer 2
+    apply assumption
+      apply(drule exE)
+       prefer 2
+      apply assumption
+    subgoal for s2 s3
+      apply(rule exI[of _ s2])
+      apply(rule exI[of _ s3])
+      apply(rule conjI)
+       apply fast
+      apply(rule conjI)
+       apply fast
+      apply(rule conjI)
+       apply auto[1]
+      apply(rule conjI)
+       apply fast
+      apply(rule conjI)
+       apply fast
+      apply(rule conjI)
+       apply fast
+      apply(rule conjI)
+       apply fast
+      apply(rule conjI)
+       apply fast
+      apply((rule allI)+)
+      apply simp
+      by (smt (verit) substate.simps(2) substate.simps(9) substate_toEnvNum_id toEnvP.simps(1))
+    using prems(5) by (simp split: if_splits)
+  apply(rule conjI)
+  using prems(1-4) prems(6) apply simp
+  apply(rule conjI)
+  using prems(1-4) prems(7) apply simp
+  apply(rule conjI)
+  using prems(1-4) prems(8) apply simp
+   apply blast
+  apply(rule conjI)
+  using prems(1-4) prems(9) apply simp
+  apply(rule conjI)
+  using prems(1-4) prems(10) apply simp
+  apply(rule conjI)
+  using prems(1-4) prems(11) apply simp
+  apply(rule conjI)
+  using prems(1-4) prems(12) apply simp
+   apply blast
+  apply(rule conjI)
+  using prems(1-4) prems(13) apply simp
+  apply(rule conjI)
+  using prems(1-4) prems(14) substate_refl apply simp
+  apply(rule conjI)
+  using prems(1-4) prems(15) apply simp
+  apply(rule conjI)
+  using prems(1-4) prems(16) apply simp
+  using prems(1-4) prems(17) by simp
+  done
+
+end
