case-studies/revolvingDoor/Extra6.thy
@@ -1,0 +1,118 @@
+theory Extra6
+  imports ExtraInv VCTheoryLemmas
+begin
+
+theorem extra6: "VC6 extraInv env s0 userValue pressure_value"
+  apply(simp only: VC6_def extraInv_def)
+  apply(rule impI)
+  apply(rule conjI)
+   apply simp
+  apply((drule conjE)+)
+                   prefer 18
+                   apply assumption
+                  prefer 17
+                  apply assumption
+                 prefer 16
+                 apply assumption
+                prefer 15
+                apply assumption
+               prefer 14
+               apply assumption
+              prefer 13
+              apply assumption
+             prefer 12
+             apply assumption
+            prefer 11
+            apply assumption
+           prefer 10
+           apply assumption
+          prefer 9
+          apply assumption
+         prefer 8
+         apply assumption
+        prefer 7
+        apply assumption
+       prefer 6
+       apply assumption
+      prefer 5
+      apply assumption
+     prefer 4
+     apply assumption
+    prefer 3
+    apply assumption
+   prefer 2
+   apply assumption
+  subgoal premises prems
+    apply(rule conjI)
+    using prems(1-5) prems(6) apply simp
+    apply(rule conjI)
+    using prems(1-5) prems(7) apply simp
+    apply(rule conjI)
+    using prems(1-5) prems(8) apply simp
+    apply(rule conjI)
+    using prems(1-5) prems(9) apply simp
+     apply blast
+    apply(rule conjI)
+    using prems(1-5) prems(10) apply simp
+    apply(rule conjI)
+    using prems(1-5) prems(11) apply simp
+    apply(rule conjI)
+    using prems(1-5) prems(12) apply -[1]
+     apply(rule allI)
+     apply(rule impI)
+    subgoal for s1
+      apply(cases "s1 =  (toEnv
+       (setPstate (setVarBool (setVarBool (setVarAny s0 userValue pressure_value) rotation False) brake True) ERROR
+         Controller'suspended))")
+       apply(rule exI[of _ s0])
+      apply(rule exI[of _ " (toEnv
+       (setPstate (setVarBool (setVarBool (setVarAny s0 userValue pressure_value) rotation False) brake True) ERROR
+         Controller'suspended))"])
+      using substate_refl toEnvNum_id  apply simp
+      by (simp split: if_splits)
+    apply(rule conjI)
+    using prems(1-5) prems(13) apply -[1]
+     apply((rule allI)+)
+     apply(rule impI)
+      apply(simp split: if_splits)
+    apply(rule cut_rl[of "s0 =  (toEnv
+          (setPstate (setVarBool (setVarBool (setVarAny s0 userValue True) rotation False) brake True) user Controller'suspended))"])
+       apply simp
+    apply(rule cut_rl[of "substate s0  (toEnv
+          (setPstate (setVarBool (setVarBool (setVarAny s0 userValue True) rotation False) brake True) user Controller'suspended))"])
+    using substate_trans substate_asym apply blast
+    using substate_refl apply simp
+     apply blast
+    apply(rule conjI)
+    using prems(1-5) prems(14) apply -[1]
+     apply(rule allI)
+     apply(rule impI)
+    subgoal for s1
+      apply(cases "s1= (toEnv
+       (setPstate (setVarBool (setVarBool (setVarAny s0 userValue pressure_value) rotation False) brake True) ERROR
+         Controller'suspended))") 
+      apply(rule exI[of _ s0])
+      apply(rule exI[of _ " (toEnv
+       (setPstate (setVarBool (setVarBool (setVarAny s0 userValue pressure_value) rotation False) brake True) ERROR
+         Controller'suspended))"])
+      using substate_refl toEnvNum_id  apply (simp)
+       apply(rule allI)
+      apply((rule impI)+)
+   apply(rule cut_rl[of "s0 =  (toEnv
+          (setPstate (setVarBool (setVarBool (setVarAny s0 userValue True) rotation False) brake True) user Controller'suspended))"])
+       apply simp
+    apply(rule cut_rl[of "substate s0  (toEnv
+          (setPstate (setVarBool (setVarBool (setVarAny s0 userValue True) rotation False) brake True) user Controller'suspended))"])
+    using substate_trans substate_asym apply blast
+    using substate_refl apply simp
+    by (simp split: if_splits)
+  apply(rule conjI)
+  using prems(1-5) prems(15) apply simp
+  apply(rule conjI)
+  using prems(1-5) prems(16) apply simp
+  apply(rule conjI)
+  using prems(1-5) prems(15) prems(17) apply simp
+  using prems(1-5) prems(18) by simp
+  done
+
+end
